Hybrid_Programs/Verification_Examples/ARCH2022_Examples.thy
@@ -137,13 +137,11 @@ lemma "\<^bold>{x \<ge> 0 \<and> y \<ge> 1\<^bold>} x ::= x + 1; ((LOOP x ::= x 
   apply (rule hoare_kcomp[where R="(x \<ge> 1 \<and> y \<ge> 1)\<^sup>e"])
    apply (rule hoare_kcomp[where R="(x \<ge> 1 \<and> y \<ge> 1)\<^sup>e"])
     apply (rule hoare_choice)
-     \<comment> \<open> Use the fact that y is outside the frame of the loop to preserve its invariants \<close>
-     apply (rule nmods_frame_law[where a="{y}\<^sub>v"])
-       apply (rule nmods_loop)
-        apply (simp)
-       apply (rule nmods_assign)
-         apply (simp_all add: unrest)
-      apply unrest
+    \<comment> \<open> Use the fact that y is outside the frame of the loop to preserve its invariants \<close>
+     apply (rule nmods_frame_law)
+      apply (rule nmods_loop)
+      apply (rule nmods_assign)
+      apply (subst_eval)
      apply (rule hoare_loopI)
        apply (hoare_wp_auto)
       apply (expr_auto)
@@ -166,10 +164,10 @@ lemma "\<^bold>{x > 0 \<and> y > 0\<^bold>} {x` = 5} ; (LOOP x::=x+3 INV (x > 0)
 proof -
   have "\<^bold>{x > 0 \<and> y > 0\<^bold>} {x` = 5} ; (LOOP x::=x+3 INV (x > 0) \<sqinter> y::=x) \<^bold>{x > 0 \<and> y > 0\<^bold>}"
     apply (rule hoare_kcomp_inv)
-   apply (dInduct_mega)
+     apply (dInduct_mega)
     apply (rule hoare_choice)
-     apply (rule nmods_frame_law[where a="{y}\<^sub>v"])
-    apply (simp add: closure, unrest)
+     apply (rule nmods_frame_law)
+      apply (rule nmods_loop, rule nmods_assign, subst_eval)
      apply (rule hoare_loopI)
        apply (hoare_wp_auto)
       apply expr_auto
@@ -2228,7 +2226,7 @@ lemma "`(v \<ge> 0 \<and> A > 0 \<and> B \<ge> b \<and> b > 0 \<and> \<epsilon> 
               apply (simp only: fbox_diff_inv_on)
               apply (diff_inv_on_single_ineq_intro "(0)\<^sup>e" "(1)\<^sup>e"; (force | vderiv))
              apply (rule diff_weak_on_rule, expr_simp)
-    by (diff_inv_on_eq | (rule nmods_invariant[OF nmods_g_orbital_on_discrete']; expr_simp))+
+    by (diff_inv_on_eq | (rule nmods_invariant; (auto intro!: closure simp add: subst_eval)))+
       (clarsimp simp: le_fun_def)+
   apply (rule_tac C="(-c * v + a*c\<^sup>2/2 \<le> y - y0 \<and> y - y0 \<le> c * v - a*c\<^sup>2/2)\<^sup>e" in diff_cut_on_rule)
   subgoal for v0 y0
